src/ADTNotation/BuildComputationalADT.v
@@ -20,11 +20,11 @@ Delimit Scope cADT_scope with cADT.
 (* Notations for computational ADT methods. *)
 
 Record cMethDef {Rep : Type} (Sig : methSig) :=
-  { cMethBody :> cMethodType Rep (methDom Sig) (methCod Sig)}.
+  { cMethBody :> cMethodType (methArity Sig) Rep (methDom Sig) (methCod Sig)}.
 
 Notation "'Def' 'Method0' id r .. xn : 'rep' '*' cod := bod" :=
   (Build_cMethDef
-     {| methID := id; methDom := [ ] ; methCod := Some (cod : Type) |}
+     {| methID := id; methArity := 1; methDom := [ ] ; methCod := Some (cod : Type) |}
      (fun r => .. (fun xn =>
                      let _ := {| codHint := Some (cod : Type) |} in
                      (bod%comp : cMethodType' _ [ ] codHint )) ..))
@@ -36,7 +36,7 @@ Notation "'Def' 'Method0' id r .. xn : 'rep' '*' cod := bod" :=
 
 Notation "'Def' 'Method1' id r .. xn : 'rep' '*' cod := bod" :=
   (Build_cMethDef
-     {| methID := id; methDom := [ _ ] ; methCod := Some (cod : Type) |}
+     {| methID := id; methArity := 1; methDom := [ _ ] ; methCod := Some (cod : Type) |}
      (fun r => .. (fun xn =>
                      let _ := {| codHint := Some (cod : Type) |} in
                      (bod%comp : cMethodType' _ [ ] codHint )) ..))
@@ -48,7 +48,7 @@ Notation "'Def' 'Method1' id r .. xn : 'rep' '*' cod := bod" :=
 
 Notation "'Def' 'Method2' id r .. xn : 'rep' '*' cod := bod" :=
   (Build_cMethDef
-     {| methID := id; methDom := [ _; _ ] ; methCod := Some (cod : Type) |}
+     {| methID := id; methArity := 1; methDom := [ _; _ ] ; methCod := Some (cod : Type) |}
      (fun r => .. (fun xn =>
                      let _ := {| codHint := Some (cod : Type) |} in
                      (bod%comp : cMethodType' _ [ ] codHint )) ..))
@@ -60,7 +60,7 @@ Notation "'Def' 'Method2' id r .. xn : 'rep' '*' cod := bod" :=
 
 Notation "'Def' 'Method3' id r .. xn : 'rep' '*' cod := bod" :=
   (Build_cMethDef
-     {| methID := id; methDom := [ _; _; _ ] ; methCod := Some (cod : Type) |}
+     {| methID := id; methArity := 1; methDom := [ _; _; _ ] ; methCod := Some (cod : Type) |}
      (fun r => .. (fun xn =>
                      let _ := {| codHint := Some (cod : Type) |} in
                      (bod%comp : cMethodType' _ [ ] codHint )) ..))
@@ -72,7 +72,7 @@ Notation "'Def' 'Method3' id r .. xn : 'rep' '*' cod := bod" :=
 
 Notation "'Def' 'Method4' id r .. xn : 'rep' '*' cod := bod" :=
   (Build_cMethDef
-     {| methID := id; methDom := [_; _; _; _ ] ; methCod := Some (cod : Type) |}
+     {| methID := id; methArity := 1; methDom := [_; _; _; _ ] ; methCod := Some (cod : Type) |}
      (fun r => .. (fun xn =>
                      let _ := {| codHint := Some (cod : Type) |} in
                      (bod%comp : cMethodType' _ [ ] codHint )) ..))
@@ -84,7 +84,7 @@ Notation "'Def' 'Method4' id r .. xn : 'rep' '*' cod := bod" :=
 
 Notation "'Def' 'Method5' id r .. xn : 'rep' '*' cod := bod" :=
   (Build_cMethDef
-     {| methID := id; methDom := [_; _; _; _; _ ] ; methCod := Some (cod : Type) |}
+     {| methID := id; methArity := 1; methDom := [_; _; _; _; _ ] ; methCod := Some (cod : Type) |}
      (fun r => .. (fun xn =>
                      let _ := {| codHint := Some (cod : Type) |} in
                      (bod%comp : cMethodType' _ [ ] codHint )) ..))
@@ -97,7 +97,7 @@ Notation "'Def' 'Method5' id r .. xn : 'rep' '*' cod := bod" :=
 (* Variant Notations for methods that don't return a value. *)
 
 Notation "'Def' 'Method0' id r .. xn : 'rep' := bod" :=
-  (Build_cMethDef {| methID := id; methDom := [ ] ; methCod := None |} (fun r => .. (fun xn => let _ := {| codHint := None |} in (bod%comp : cMethodType' _ [ ] codHint )) ..))
+  (Build_cMethDef {| methID := id; methArity := 1; methDom := [ ] ; methCod := None |} (fun r => .. (fun xn => let _ := {| codHint := None |} in (bod%comp : cMethodType' _ [ ] codHint )) ..))
     (no associativity, id at level 0, r closed binder , xn closed binder,
      only parsing,
      at level 94,
@@ -105,7 +105,7 @@ Notation "'Def' 'Method0' id r .. xn : 'rep' := bod" :=
   : cMethDefParsing_scope.
 
 Notation "'Def' 'Method1' id r .. xn : 'rep' := bod" :=
-  (Build_cMethDef {| methID := id; methDom := [_ ] ; methCod := None |} (fun r => .. (fun xn => let _ := {| codHint := None |} in (bod%comp : cMethodType' _ [ ] codHint )) ..))
+  (Build_cMethDef {| methID := id; methArity := 1; methDom := [_ ] ; methCod := None |} (fun r => .. (fun xn => let _ := {| codHint := None |} in (bod%comp : cMethodType' _ [ ] codHint )) ..))
     (no associativity, id at level 0, r closed binder , xn closed binder,
      only parsing,
      at level 94,
@@ -113,7 +113,7 @@ Notation "'Def' 'Method1' id r .. xn : 'rep' := bod" :=
   : cMethDefParsing_scope.
 
 Notation "'Def' 'Method2' id r .. xn : 'rep' := bod" :=
-  (Build_cMethDef {| methID := id; methDom := [_; _ ] ; methCod := None |} (fun r => .. (fun xn => let _ := {| codHint := None |} in (bod%comp : cMethodType' _ [ ] codHint )) ..))
+  (Build_cMethDef {| methID := id; methArity := 1; methDom := [_; _ ] ; methCod := None |} (fun r => .. (fun xn => let _ := {| codHint := None |} in (bod%comp : cMethodType' _ [ ] codHint )) ..))
     (no associativity, id at level 0, r closed binder , xn closed binder,
      only parsing,
      at level 94,
@@ -121,7 +121,7 @@ Notation "'Def' 'Method2' id r .. xn : 'rep' := bod" :=
   : cMethDefParsing_scope.
 
 Notation "'Def' 'Method3' id r .. xn : 'rep' := bod" :=
-  (Build_cMethDef {| methID := id; methDom := [_; _; _ ] ; methCod := None |} (fun r => .. (fun xn => let _ := {| codHint := None |} in (bod%comp : cMethodType' _ [ ] codHint )) ..))
+  (Build_cMethDef {| methID := id; methArity := 1; methDom := [_; _; _ ] ; methCod := None |} (fun r => .. (fun xn => let _ := {| codHint := None |} in (bod%comp : cMethodType' _ [ ] codHint )) ..))
     (no associativity, id at level 0, r closed binder , xn closed binder,
      only parsing,
      at level 94,
@@ -129,7 +129,7 @@ Notation "'Def' 'Method3' id r .. xn : 'rep' := bod" :=
   : cMethDefParsing_scope.
 
 Notation "'Def' 'Method4' id r .. xn : 'rep' := bod" :=
-  (Build_cMethDef {| methID := id; methDom := [_; _; _; _] ; methCod := None |} (fun r => .. (fun xn => let _ := {| codHint := None |} in (bod%comp : cMethodType' _ [ ] codHint )) ..))
+  (Build_cMethDef {| methID := id; methArity := 1; methDom := [_; _; _; _] ; methCod := None |} (fun r => .. (fun xn => let _ := {| codHint := None |} in (bod%comp : cMethodType' _ [ ] codHint )) ..))
     (no associativity, id at level 0, r closed binder , xn closed binder,
      only parsing,
      at level 94,
@@ -137,7 +137,7 @@ Notation "'Def' 'Method4' id r .. xn : 'rep' := bod" :=
   : cMethDefParsing_scope.
 
 Notation "'Def' 'Method5' id r .. xn : 'rep' := bod" :=
-  (Build_cMethDef {| methID := id; methDom := [_; _; _; _; _] ; methCod := None |} (fun r => .. (fun xn => let _ := {| codHint := None |} in (bod%comp : cMethodType' _ [ ] codHint )) ..))
+  (Build_cMethDef {| methID := id; methArity := 1; methDom := [_; _; _; _; _] ; methCod := None |} (fun r => .. (fun xn => let _ := {| codHint := None |} in (bod%comp : cMethodType' _ [ ] codHint )) ..))
     (no associativity, id at level 0, r closed binder , xn closed binder,
      only parsing,
      at level 94,
@@ -146,7 +146,7 @@ Notation "'Def' 'Method5' id r .. xn : 'rep' := bod" :=
 
 (* Again, pretty printing involves fewer rules. *)
 Notation "'Def' 'Method' id ( r : 'rep' ) : 'rep' '*' cod := bod" :=
-  (Build_cMethDef {| methID := id; methDom := [] ; methCod := Some cod |} (fun r => bod%comp ))
+  (Build_cMethDef {| methID := id; methArity := 1; methDom := [] ; methCod := Some cod |} (fun r => bod%comp ))
     (no associativity, id at level 0, r at level 0,
      cod at level 0,
      at level 94,
@@ -154,7 +154,7 @@ Notation "'Def' 'Method' id ( r : 'rep' ) : 'rep' '*' cod := bod" :=
   : cMethDef_scope.
 
 Notation "'Def' 'Method' id ( r : 'rep' ) x1 .. xn : 'rep' '*' cod := bod" :=
-  (Build_cMethDef {| methID := id; methDom := _ :: _ ; methCod := Some cod |} (fun r =>
+  (Build_cMethDef {| methID := id; methArity := 1; methDom := _ :: _ ; methCod := Some cod |} (fun r =>
                                                                              (fun x1 => .. (fun xn => (bod%comp )) ..)))
     (no associativity, id at level 0, r at level 0, x1 closed binder , xn closed binder,
      at level 94,
@@ -162,14 +162,14 @@ Notation "'Def' 'Method' id ( r : 'rep' ) x1 .. xn : 'rep' '*' cod := bod" :=
   : cMethDef_scope.
 
 Notation "'Def' 'Method' id ( r : 'rep' ) : 'rep' := bod" :=
-  (Build_cMethDef {| methID := id; methDom := [] ; methCod := None |} (fun r => bod%comp ))
+  (Build_cMethDef {| methID := id; methArity := 1; methDom := [] ; methCod := None |} (fun r => bod%comp ))
     (no associativity, id at level 0, r at level 0,
      at level 94,
      format "'Def'  'Method'  id  ( r  :  'rep' )  :  'rep'  :=  '/' '[  '   bod ']' ")
   : cMethDef_scope.
 
 Notation "'Def' 'Method' id ( r : 'rep' ) x1 .. xn : 'rep' := bod" :=
-  (Build_cMethDef {| methID := id; methDom := _ :: _ ; methCod := None |} (fun r =>
+  (Build_cMethDef {| methID := id; methArity := 1; methDom := _ :: _ ; methCod := None |} (fun r =>
                                                                          (fun x1 => .. (fun xn => (bod%comp )) ..)))
     (no associativity, id at level 0, r at level 0, x1 closed binder , xn closed binder,
      at level 94,
@@ -179,116 +179,104 @@ Notation "'Def' 'Method' id ( r : 'rep' ) x1 .. xn : 'rep' := bod" :=
 Delimit Scope cMethDefParsing_scope with cMethDefParsing.
 Delimit Scope cMethDef_scope with cMethDef.
 
-Record cConsDef {Rep : Type} (Sig : consSig) :=
-  { cConsBody :> cConstructorType Rep (consDom Sig) }.
-
 (* Notations for parsing Constructors. Including the arity is the simplest way to
  make typechecking work. *)
 Notation "'Def' 'Constructor0' id : 'rep' := bod" :=
-  (Build_cConsDef _ {| consID := id; consDom := [] |} ((bod%comp : cConstructorType rep [ ]) ))
+  (Build_cMethDef _ {| methID := id; methArity := 1; methDom := []; methCod := None |} ((bod%comp : cConstructorType rep [ ]) ))
     (no associativity, at level 94, id at level 0,
      format "'Def'  'Constructor0'  id  :  'rep'  :=  '/' '[  '   bod ']' " ) :
-    cConsDef_scope.
+    cMethDef_scope.
 
 Notation "'Def' 'Constructor1' id x1 .. xn : 'rep' := bod" :=
-  (Build_cConsDef _ {| consID := id; consDom := [_] |} ((fun x1 => .. ((fun xn => (bod%comp : cConstructorType rep [ ]) )) ..)))
+  (Build_cMethDef _ {| methID := id; methArity := 1; methDom := [_] ; methCod := None |} ((fun x1 => .. ((fun xn => (bod%comp : cConstructorType rep [ ]) )) ..)))
     (no associativity, at level 94, id at level 0,
      x1 closed binder, xn closed binder,
      format "'Def'  'Constructor1'  id  x1  ..  xn  :  'rep'  :=  '/' '[  '   bod ']' " ) :
-    cConsDef_scope.
+    cMethDef_scope.
 
 Notation "'Def' 'Constructor2' id x1 .. xn : 'rep' := bod" :=
-  (Build_cConsDef _ {| consID := id; consDom := [_; _] |} ((fun x1 => .. ((fun xn => (bod%comp : cConstructorType rep [ ]) )) ..)))
+  (Build_cMethDef _ {| methID := id; methArity := 1; methDom := [_; _] ; methCod := None |} ((fun x1 => .. ((fun xn => (bod%comp : cConstructorType rep [ ]) )) ..)))
     (no associativity, at level 94, id at level 0,
      x1 closed binder, xn closed binder,
      format "'Def'  'Constructor2'  id  x1  ..  xn  :  'rep'  :=  '/' '[  '   bod ']' " ) :
-    cConsDef_scope.
+    cMethDef_scope.
 
 Notation "'Def' 'Constructor3' id x1 .. xn : 'rep' := bod" :=
-  (Build_cConsDef _ {| consID := id; consDom := [_; _; _] |} ((fun x1 => .. ((fun xn => (bod%comp : cConstructorType rep [ ]) )) ..)))
+  (Build_cMethDef _ {| methID := id; methArity := 1; methDom := [_; _; _] ; methCod := None |} ((fun x1 => .. ((fun xn => (bod%comp : cConstructorType rep [ ]) )) ..)))
     (no associativity, at level 94, id at level 0,
      x1 closed binder, xn closed binder,
      format "'Def'  'Constructor3'  id  x1  ..  xn  :  'rep'  :=  '/' '[  '   bod ']' " ) :
-    cConsDef_scope.
+    cMethDef_scope.
 
 Notation "'Def' 'Constructor4' id x1 .. xn : 'rep' := bod" :=
-  (Build_cConsDef _ {| consID := id; consDom := [_; _; _ ; _] |} ((fun x1 => .. ((fun xn => (bod%comp : cConstructorType rep [ ]) )) ..)))
+  (Build_cMethDef _ {| methID := id; methArity := 1; methDom := [_; _; _ ; _] ; methCod := None |} ((fun x1 => .. ((fun xn => (bod%comp : cConstructorType rep [ ]) )) ..)))
     (no associativity, at level 94, id at level 0,
      x1 closed binder, xn closed binder,
      format "'Def'  'Constructor4'  id  x1  ..  xn  :  'rep'  :=  '/' '[  '   bod ']' " ) :
-    cConsDef_scope.
+    cMethDef_scope.
 
 Notation "'Def' 'Constructor5' id x1 .. xn : 'rep' := bod" :=
-  (Build_cConsDef _ {| consID := id; consDom := [_; _; _; _; _] |} ((fun x1 => .. ((fun xn => (bod%comp : cConstructorType rep [ ]) )) ..)))
+  (Build_cMethDef _ {| methID := id; methArity := 1; methDom := [_; _; _; _; _] ; methCod := None |} ((fun x1 => .. ((fun xn => (bod%comp : cConstructorType rep [ ]) )) ..)))
     (no associativity, at level 94, id at level 0,
      x1 closed binder, xn closed binder,
      format "'Def'  'Constructor5'  id  x1  ..  xn  :  'rep'  :=  '/' '[  '   bod ']' " ) :
-    cConsDef_scope.
+    cMethDef_scope.
 
 Notation "'Def' 'Constructor6' id x1 .. xn : 'rep' := bod" :=
-  (Build_cConsDef _ {| consID := id; consDom := [_; _; _; _;_; _] |} ((fun x1 => .. ((fun xn => (bod%comp : cConstructorType rep [ ]) )) ..)))
+  (Build_cMethDef _ {| methID := id; methArity := 1; methDom := [_; _; _; _;_; _] ; methCod := None |} ((fun x1 => .. ((fun xn => (bod%comp : cConstructorType rep [ ]) )) ..)))
     (no associativity, at level 94, id at level 0,
      x1 closed binder, xn closed binder,
      format "'Def'  'Constructor6'  id  x1  ..  xn  :  'rep'  :=  '/' '[  '   bod ']' " ) :
-    cConsDef_scope.
+    cMethDef_scope.
 
 Notation "'Def' 'Constructor7' id x1 .. xn : 'rep' := bod" :=
-  (Build_cConsDef _ {| consID := id; consDom := [_; _; _; _; _; _; _] |} ((fun x1 => .. ((fun xn => (bod%comp : cConstructorType rep [ ]) )) ..)))
+  (Build_cMethDef _ {| methID := id; methArity := 1; methDom := [_; _; _; _; _; _; _] ; methCod := None |} ((fun x1 => .. ((fun xn => (bod%comp : cConstructorType rep [ ]) )) ..)))
     (no associativity, at level 94, id at level 0,
      x1 closed binder, xn closed binder,
      format "'Def'  'Constructor7'  id  x1  ..  xn  :  'rep'  :=  '/' '[  '   bod ']' " ) :
-    cConsDef_scope.
+    cMethDef_scope.
 
 Notation "'Def' 'Constructor8' id x1 .. xn : 'rep' := bod" :=
-  (Build_cConsDef _ {| consID := id; consDom := [_; _; _; _; _; _; _ ; _] |} ((fun x1 => .. ((fun xn => (bod%comp : cConstructorType rep [ ]) )) ..)))
+  (Build_cMethDef _ {| methID := id; methArity := 1; methDom := [_; _; _; _; _; _; _ ; _] ; methCod := None |} ((fun x1 => .. ((fun xn => (bod%comp : cConstructorType rep [ ]) )) ..)))
     (no associativity, at level 94, id at level 0,
      x1 closed binder, xn closed binder,
      format "'Def'  'Constructor8'  id  x1  ..  xn  :  'rep'  :=  '/' '[  '   bod ']' " ) :
-    cConsDef_scope.
+    cMethDef_scope.
 
 Notation "'Def' 'Constructor9' id x1 .. xn : 'rep' := bod" :=
-  (Build_cConsDef _ {| consID := id; consDom := [_; _; _; _; _; _; _; _; _] |} ((fun x1 => .. ((fun xn => (bod%comp : cConstructorType rep [ ]) )) ..)))
+  (Build_cMethDef _ {| methID := id; methArity := 1; methDom := [_; _; _; _; _; _; _; _; _] ; methCod := None |} ((fun x1 => .. ((fun xn => (bod%comp : cConstructorType rep [ ]) )) ..)))
     (no associativity, at level 94, id at level 0,
      x1 closed binder, xn closed binder,
      format "'Def'  'Constructor9'  id  x1  ..  xn  :  'rep'  :=  '/' '[  '   bod ']' " ) :
-    cConsDef_scope.
+    cMethDef_scope.
 
 Notation "'Def' 'Constructor10' id x1 .. xn : 'rep' := bod" :=
-  (Build_cConsDef _ {| consID := id; consDom := [_; _; _; _; _; _; _; _;  _; _] |} ((fun x1 => .. ((fun xn => (bod%comp : cConstructorType rep [ ]) )) ..)))
+  (Build_cMethDef _ {| methID := id; methArity := 1; methDom := [_; _; _; _; _; _; _; _;  _; _] ; methCod := None |} ((fun x1 => .. ((fun xn => (bod%comp : cConstructorType rep [ ]) )) ..)))
     (no associativity, at level 94, id at level 0,
      x1 closed binder, xn closed binder,
      format "'Def'  'Constructor10'  id  x1  ..  xn  :  'rep'  :=  '/' '[  '   bod ']' " ) :
-    cConsDef_scope.
+    cMethDef_scope.
 
 (* Once the type infomation is in hand, two rules can handle pretty printing.  *)
 Notation "'Def' 'Constructor' id x1 .. xn : 'rep' := bod" :=
-  (Build_cConsDef _ {| consID := id; consDom := _ |} ((fun x1 => .. ((fun xn => bod%comp )) ..)))
+  (Build_cMethDef _ {| methID := id; methArity := 1; methDom := _ ; methCod := None |} ((fun x1 => .. ((fun xn => bod%comp )) ..)))
     (no associativity, at level 94, id at level 0,
      x1 closed binder, xn closed binder,
      format "'Def'  'Constructor'  id  x1  ..  xn  :  'rep'  :=  '/' '[  '   bod ']' " ) :
-    cConsDef_scope.
+    cMethDef_scope.
 
 Notation "'Def' 'Constructor' id : 'rep' := bod" :=
-  (Build_cConsDef _ {| consID := id; consDom := [] |} bod%comp)
+  (Build_cMethDef _ {| methID := id; methArity := 1; methDom := [] ; methCod := None |} bod%comp)
     (no associativity, at level 94, id at level 0,
      format "'Def'  'Constructor'  id :  'rep'  :=  '/' '[  '   bod ']' " ) :
-    cConsDef_scope.
+    cMethDef_scope.
 
-Delimit Scope cConsDef_scope with cConsDef.
+Delimit Scope cMethDef_scope with cMethDef.
 
 (* Lookup functions for constructor and method definitions. Because
    these definitions are parameterized on a signature, their
    bodies are contained in an indexed list [ilist] which is
    parameterized on a list of those signatures. *)
-
-Definition getcConsDef
-           (Rep : Type)
-           {n}
-        (consSigs : Vector.t consSig n)
-        (consDefs : ilist (B := @cConsDef Rep) consSigs)
-        (idx : Fin.t n)
-: cConstructorType Rep (consDom (Vector.nth consSigs idx)) :=
-  cConsBody (ith consDefs idx).
 
 Definition getcMethDef
            (Rep : Type)
@@ -297,14 +285,14 @@ Definition getcMethDef
            (methDefs : ilist methSigs)
            (idx : Fin.t n)
   : cMethodType
+      (methArity (Vector.nth methSigs idx))
       Rep
       (methDom (Vector.nth methSigs idx))
       (methCod (Vector.nth methSigs idx)) :=
   cMethBody (ith methDefs idx).
 
 (* Always simplify method lookup when the index is specified. *)
-Arguments getcConsDef [_] {n} [_] _ idx%string / .
-Arguments getcMethDef [_] {n} [_] _ idx%string / _ .
+Arguments getcMethDef [_] {n} [_] _ idx%string / .
 
 (* [BuildcADT] constructs an computational ADT from a single constructor
    definition and a list of method signatures,
@@ -314,23 +302,13 @@ Definition DecoratedcADT (dSig : DecoratedADTSig) := cADT dSig.
 
 Program Definition BuildcADT
         {Rep : Type}
-        {n n'}
-        {consSigs : Vector.t consSig n}
+        {n'}
         {methSigs : Vector.t methSig n'}
-        (consDefs : ilist (B := @cConsDef Rep) consSigs)
         (methDefs : ilist (B:= @cMethDef Rep) methSigs)
-: DecoratedcADT (BuildADTSig consSigs methSigs)
+: DecoratedcADT (BuildADTSig methSigs)
       := existT _ Rep {|
-                  pcConstructors idx := getcConsDef consDefs idx;
                   pcMethods idx := getcMethDef methDefs idx
                 |}.
-
-Definition callcADTConstructor
-           {dSig : DecoratedADTSig}
-           (adt : DecoratedcADT dSig)
-           (idxMap : BoundedIndex (ConstructorNames dSig) -> ConstructorIndex dSig)
-           (idx : BoundedIndex (ConstructorNames dSig))
-  := cConstructors adt (idxMap idx).
 
 Definition callcADTMethod
            {dSig : DecoratedADTSig}
@@ -341,28 +319,22 @@ Definition callcADTMethod
 
 (* Notation for ADTs built from [BuildADT]. *)
 
-Notation "'cADTRep' r { cons1 , meth1 , .. , methn } " :=
+Notation "'cADTRep' r { meth1 , .. , methn } " :=
   (let _ := {| rep := r |} in
     @BuildcADT r
              _ _
-             _ _
-             (icons cons1%cConsDef (@inil _ (@cConsDef r)))
              (icons meth1%cMethDefParsing .. (icons methn%cMethDefParsing (@inil _ (@cMethDef r))) ..))
     (no associativity, at level 96, r at level 0,
-     format "'cADTRep'  r  '/' '[hv  ' {  cons1 ,  '//' meth1 , '//' .. , '//' methn  ']' }") :
+     format "'cADTRep'  r  '/' '[hv  ' {  meth1 , '//' .. , '//' methn  ']' }") :
     ADTParsing_scope.
 
-Notation "'cADTRep' r { cons1 , meth1 , .. , methn } " :=
+Notation "'cADTRep' r { meth1 , .. , methn } " :=
   (@BuildcADT r
              _ _
-             _ _
-             (icons cons1%cConsDef (@inil _ (@cConsDef r)))
              (icons meth1%cMethDef .. (icons methn%cMethDef (@inil _  (@cMethDef r))) ..))
     (no associativity, at level 96, r at level 0,
-     format "'cADTRep'  r  '/' '[hv  ' {  cons1 , '//' meth1 , '//' .. , '//' methn  ']' }") : ADT_scope.
+     format "'cADTRep'  r  '/' '[hv  ' {  meth1 , '//' .. , '//' methn  ']' }") : ADT_scope.
 
 (* Notations for method calls. *)
 Notation CallMethod CompADT idx := (callcADTMethod CompADT (fun idx => ibound (indexb idx))
-                                                  {| bindex := idx |}).
-Notation CallConstructor CompADT idx := (callcADTConstructor CompADT (fun idx => ibound (indexb idx))
                                                   {| bindex := idx |}).
