src/ADTRefinement/GeneralBuildADTRefinements.v
@@ -19,201 +19,24 @@ Section BuildADTRefinements.
   Require Import Coq.Strings.String.
   Local Hint Resolve string_dec.
 
-  Lemma refineADT_BuildADT_ReplaceConstructor
-        (Rep : Type)
-        (AbsR : Rep -> Rep -> Prop)
-        {n n'}
-        (consSigs : Vector.t consSig n)
-        (methSigs : Vector.t methSig n')
-        (consDefs : ilist (B := @consDef Rep) consSigs)
-        (methDefs : ilist (B := @methDef Rep) methSigs)
-        (idx : @Fin.t n)
-        (newDef : consDef (Vector.nth consSigs idx))
-  :
-    (forall consIdx,
-       refineConstructor AbsR (getConsDef consDefs consIdx) (getConsDef consDefs consIdx))
-    -> (forall methIdx,
-          refineMethod AbsR (getMethDef methDefs methIdx) (getMethDef methDefs methIdx))
-    -> refineConstructor AbsR
-                         (consBody (ith consDefs idx ))
-                         (consBody newDef)
-    -> refineADT
-         (BuildADT consDefs methDefs)
-         (ADTReplaceConsDef consDefs methDefs idx newDef).
-  Proof.
-    intros; eapply refineADT_BuildADT_Rep with (AbsR := AbsR); eauto.
-    intros; unfold getConsDef.
-    unfold replaceConsDef.
-    destruct (fin_eq_dec consIdx idx); subst.
-    rewrite ith_replace_Index_eq; eauto.
-    rewrite ith_replace_Index_neq; eauto.
-  Qed.
-
-  Corollary SharpenStep_BuildADT_ReplaceConstructor_eq
-            (Rep : Type)
-            {n n'}
-            (consSigs : Vector.t consSig n)
-            (methSigs : Vector.t methSig n')
-            (consDefs : ilist (B := @consDef Rep) consSigs)
-            (methDefs : ilist (B := @methDef Rep) methSigs)
-            (idx : @Fin.t n)
-            (newDef : consDef (Vector.nth consSigs idx))
-            adt''
-    :
-    (let H := consBody newDef in refineConstructor eq (consBody (ith consDefs idx)) H)
-    -> refineADT (ADTReplaceConsDef consDefs methDefs idx newDef) adt''
-    -> refineADT (BuildADT consDefs methDefs) adt''.
-  Proof.
-    intros; eapply SharpenStep; try exact X.
-    eapply refineADT_BuildADT_ReplaceConstructor with (AbsR := eq);
-    simpl; unfold refine; intros; subst; eauto.
-    - reflexivity.
-    - reflexivity.
-  Qed.
-
-  Corollary FullySharpenStep_BuildADT_ReplaceConstructor_eq
-            (Rep : Type)
-            {n n'}
-            (consSigs : Vector.t consSig n)
-            (methSigs : Vector.t methSig n')
-            (consDefs : ilist (B := @consDef Rep) consSigs)
-            (methDefs : ilist (B := @methDef Rep) methSigs)
-            (idx : @Fin.t n)
-            (newDef : consDef (Vector.nth consSigs idx))
-            adt''
-    :
-      (let H := consBody newDef in refineConstructor eq (consBody (ith consDefs idx)) H)
-    -> FullySharpenedUnderDelegates (ADTReplaceConsDef consDefs methDefs idx newDef) adt''
-    -> FullySharpenedUnderDelegates (BuildADT consDefs methDefs) adt''.
-  Proof.
-    intros; eapply FullySharpenStep; try exact X.
-    eapply refineADT_BuildADT_ReplaceConstructor with (AbsR := eq);
-    simpl; unfold refine; intros; subst; eauto.
-    - reflexivity.
-    - reflexivity.
-  Qed.
-
-  (*Corollary SharpenStep_BuildADT_ReplaceConstructor_eq
-            (Rep : Type)
-            (consSigs : list consSig)
-            (methSigs : list methSig)
-            (consDefs : ilist (@consDef Rep) consSigs)
-            (methDefs : ilist (@methDef Rep) methSigs)
-            (idx : @BoundedString (List.map consID consSigs))
-            (newDef : consDef (nth_Bounded consID consSigs idx))
-  :
-    (forall d,
-       refine (consBody (ith_Bounded consID consDefs idx) d) (consBody newDef d))
-    -> Sharpened (ADTReplaceConsDef consDefs methDefs idx newDef)
-    -> Sharpened (BuildADT consDefs methDefs).
-  Proof.
-    intros; eapply SharpenStep; eauto.
-    apply refineADT_BuildADT_ReplaceConstructor_eq; eauto.
-  Defined. *)
-
-  (*
-
-Definition Sect {A B : Type} (s : A -> B) (r : B -> A) :=
-  forall x : A, r (s x) = x.
-
-Class IsEquiv {A B : Type} (f : A -> B) := BuildIsEquiv {
-  equiv_inv : B -> A ;
-  eisretr : Sect equiv_inv f;
-  eissect : Sect f equiv_inv;
-  eisadj : forall x : A, eisretr (f x) = f_equal f (eissect x)
-}.
-
-Arguments eisretr {A B} f {_} _.
-Arguments eissect {A B} f {_} _.
-Arguments eisadj {A B} f {_} _.
-
-Definition apD10 {A} {B:A->Type} {f g : forall x, B x} (h:f=g)
-  : forall x, f x = g x
-  := fun x => match h with eq_refl => eq_refl end.
-
-Class Funext :=
-  { isequiv_apD10 :> forall (A : Type) (P : A -> Type) f g, IsEquiv (@apD10 A P f g) }.
-
-(* We'll just assume functional extensionality for now. *)
-Axiom IsHProp : Type -> Type.
-Existing Class IsHProp.
-Instance : forall A, IsHProp (IsHProp A).
-Admitted.
-
-Axiom allpath_hprop : forall `{H : IsHProp A} (x y : A), x = y.
-Axiom hprop_allpath : forall (A : Type), (forall (x y : A), x = y) -> IsHProp A.
-
-Global Instance trunc_forall `{P : A -> Type} `{forall a, IsHProp (P a)}
-  : IsHProp (forall a, P a) | 100.
-Admitted.
-
-Instance trunc_prod `{IsHProp A, IsHProp B} : IsHProp (A * B).
-Admitted.
-
-Record hProp := hp { hproptype :> Type ; isp : IsHProp hproptype}.
-Existing Instance isp.
-
-Instance : forall A : hProp, IsHProp A.
-Admitted.
-
-Lemma path_sig_hprop {A} {P : A -> Prop} `{forall x : A, IsHProp (P x)}
-      (x y : sig P)
-: proj1_sig x = proj1_sig y -> x = y.
-Proof.
-  destruct_head sig; intros; subst; f_equal; apply allpath_hprop.
-Defined.
-
-
-Lemma refineADT_BuildADT_ReplaceConstructor_sigma
-        (RepT : Type)
-        (RepInv : RepT -> Prop)
-        `{forall x, IsHProp (RepInv x)}
-        (consSigs : list consSig)
-        (methSigs : list methSig)
-        (consDefs : ilist (@consDef (sig RepInv)) consSigs)
-        (methDefs : ilist (@methDef (sig RepInv)) methSigs)
-        (idx : @BoundedString (List.map consID consSigs))
-        (newDef : consDef (nth_Bounded consID consSigs idx))
-  : refineConstructor (fun x y => proj1_sig x = proj1_sig y)
-                      (consBody (ith_Bounded _ consDefs idx))
-                      (consBody newDef)
-    -> refineADT
-         (BuildADT consDefs methDefs)
-         (ADTReplaceConsDef consDefs methDefs idx newDef).
-  Proof.
-    intro H'.
-    eapply refineADT_BuildADT_ReplaceConstructor_eq.
-    simpl in *; intros; subst; eauto.
-    etransitivity; [ | eapply_hyp; reflexivity ].
-    eapply refine_bind; [ reflexivity | intro ].
-    eapply refine_flip_impl_Pick;
-      repeat intro;
-      apply path_sig_hprop;
-      assumption.
-  Qed. *)
 
   Lemma refineADT_BuildADT_ReplaceMethod
         (Rep : Type)
-        {n n'}
-        (consSigs : Vector.t consSig n)
-        (methSigs : Vector.t methSig n')
-        (consDefs : ilist (B := @consDef Rep) consSigs)
+        {n}
+        (methSigs : Vector.t methSig n)
         (methDefs : ilist (B := @methDef Rep) methSigs)
-        (idx : @Fin.t n')
+        (idx : @Fin.t n)
         (newDef : methDef (Vector.nth methSigs idx))
         AbsR
-        (AbsR_reflexive_constructor :
-           forall consIdx,
-             refineConstructor AbsR (getConsDef consDefs consIdx) (getConsDef consDefs consIdx))
         (AbsR_reflexive_method :
            forall methIdx,
-             refineMethod AbsR (getMethDef methDefs methIdx) (getMethDef methDefs methIdx))
+             refineMethod AbsR _ (getMethDef methDefs methIdx) (getMethDef methDefs methIdx))
   : refineMethod AbsR
-                 (methBody (ith methDefs idx))
+                 _ (methBody (ith methDefs idx))
                  (methBody newDef)
     -> refineADT
-         (BuildADT consDefs methDefs)
-         (ADTReplaceMethDef consDefs methDefs idx newDef).
+         (BuildADT methDefs)
+         (ADTReplaceMethDef methDefs idx newDef).
   Proof.
     intros; eapply refineADT_BuildADT_Rep with (AbsR := AbsR); trivial.
     intros; unfold getMethDef.
@@ -225,18 +48,16 @@ Lemma refineADT_BuildADT_ReplaceConstructor_sigma
 
   Corollary SharpenStep_BuildADT_ReplaceMethod_eq
         (Rep : Type)
-        {n n'}
-        (consSigs : Vector.t consSig n)
-        (methSigs : Vector.t methSig n')
-        (consDefs : ilist (B := @consDef Rep) consSigs)
+        {n}
+        (methSigs : Vector.t methSig n)
         (methDefs : ilist (B := @methDef Rep) methSigs)
-        (idx : @Fin.t n')
+        (idx : @Fin.t n)
         (newDef : methDef (Vector.nth methSigs idx))
         adt''
     :
-      (let H := methBody newDef in refineMethod eq (methBody (ith methDefs idx)) newDef)
-      -> refineADT (ADTReplaceMethDef consDefs methDefs idx newDef) adt''
-      -> refineADT (BuildADT consDefs methDefs) adt''.
+      (let H := methBody newDef in refineMethod eq _ (methBody (ith methDefs idx)) newDef)
+      -> refineADT (ADTReplaceMethDef methDefs idx newDef) adt''
+      -> refineADT (BuildADT methDefs) adt''.
   Proof.
     intros; eapply SharpenStep.
     eapply refineADT_BuildADT_ReplaceMethod with (AbsR := eq);
@@ -246,21 +67,19 @@ Lemma refineADT_BuildADT_ReplaceConstructor_sigma
 
   Lemma FullySharpenStep_BuildADT_ReplaceMethod_eq
         (Rep : Type)
-        {n n'}
-        (consSigs : Vector.t consSig n)
-        (methSigs : Vector.t methSig n')
-        (consDefs : ilist (B := @consDef Rep) consSigs)
+        {n}
+        (methSigs : Vector.t methSig n)
         (methDefs : ilist (B := @methDef Rep) methSigs)
-        (idx : @Fin.t n')
+        (idx : @Fin.t n)
         (newDef : methDef (Vector.nth methSigs idx))
         adt''
     :
-      (let H := methBody newDef in refineMethod eq (methBody (ith methDefs idx)) newDef)
+      (let H := methBody newDef in refineMethod eq _ (methBody (ith methDefs idx)) newDef)
       -> FullySharpenedUnderDelegates
-           (ADTReplaceMethDef consDefs methDefs idx newDef)
+           (ADTReplaceMethDef methDefs idx newDef)
            adt''
       -> FullySharpenedUnderDelegates
-           (BuildADT consDefs methDefs)
+           (BuildADT methDefs)
            adt''.
   Proof.
     intros; eapply FullySharpenStep.
@@ -269,72 +88,12 @@ Lemma refineADT_BuildADT_ReplaceConstructor_sigma
     exact X.
   Qed.
 
-  (*Corollary SharpenStep_BuildADT_ReplaceMethod_eq
-            (Rep : Type)
-            (consSigs : list consSig)
-            (methSigs : list methSig)
-            (consDefs : ilist (@consDef Rep) consSigs)
-            (methDefs : ilist (@methDef Rep) methSigs)
-            (idx : @BoundedString (List.map methID methSigs))
-            (newDef : methDef (nth_Bounded _ methSigs idx))
-  :
-    (forall r_n n,
-       refine (methBody (ith_Bounded methID methDefs idx) r_n n) (methBody newDef r_n n))
-    -> Sharpened (ADTReplaceMethDef consDefs methDefs idx newDef)
-    -> Sharpened (BuildADT consDefs methDefs).
-  Proof.
-    intros; eapply SharpenStep; eauto.
-    intros; eapply refineADT_BuildADT_ReplaceMethod_eq; eauto.
-  Defined. *)
-
-  (*Lemma refineADT_BuildADT_ReplaceMethod_sigma
-        (RepT : Type)
-        (RepInv : RepT -> Prop)
-        {n n'}
-        (consSigs : Vector.t consSig n)
-        (methSigs : Vector.t methSig n')
-        (consDefs : ilist (B := @consDef (sig RepInv)) consSigs)
-        (methDefs : ilist (B := @methDef (sig RepInv)) methSigs)
-        (idx : @Fin.t n')
-        (newDef : methDef (Vector.nth methSigs idx))
-        (AbsR_reflexive_method :
-           forall methIdx,
-             refineMethod (fun x y => proj1_sig x = proj1_sig y)
-                          (getMethDef methDefs methIdx)
-                          (getMethDef methDefs methIdx))
-  : refineMethod (fun x y => proj1_sig x = proj1_sig y)
-                 (methBody (ith methDefs idx))
-                 (methBody newDef)
-    -> refineADT
-         (BuildADT consDefs methDefs)
-         (ADTReplaceMethDef consDefs methDefs idx newDef).
-  Proof.
-    intro H'.
-    eapply refineADT_BuildADT_ReplaceMethod with
-    (AbsR := fun r_o r_n => proj1_sig r_o = proj1_sig r_n); eauto;
-    simpl in *; intros; subst; eauto.
-    computes_to_econstructor; eauto.
-  Qed. *)
-
-  (* Notation-Friendly Lemmas for constructing an easily extractible
-     ADT implementation. *)
-
   Definition Notation_Friendly_BuildMostlySharpenedcADT
-             {n n'}
-             {consSigs : Vector.t consSig n}
-             {methSigs : Vector.t methSig n'}
+             {n}
+             {methSigs : Vector.t methSig n}
              (DelegateIDs : nat)
              (DelegateSigs : Fin.t DelegateIDs -> ADTSig)
              (rep : (Fin.t DelegateIDs -> Type) -> Type)
-             (cConstructors :
-                forall
-                  (DelegateReps : Fin.t DelegateIDs -> Type)
-                  (DelegateImpls : forall idx,
-                                     ComputationalADT.pcADT (DelegateSigs idx) (DelegateReps idx)),
-                  ilist
-                    (B := fun Sig : consSig =>
-                            ComputationalADT.cConstructorType (rep DelegateReps) (consDom Sig))
-                    consSigs)
              (cMethods :
                 forall
                   (DelegateReps : Fin.t DelegateIDs -> Type)
@@ -342,37 +101,24 @@ Lemma refineADT_BuildADT_ReplaceConstructor_sigma
                                      ComputationalADT.pcADT (DelegateSigs idx) (DelegateReps idx)),
                   ilist
                     (B := fun Sig : methSig =>
-                       ComputationalADT.cMethodType (rep DelegateReps)
+                       ComputationalADT.cMethodType _ (rep DelegateReps)
                                                     (methDom Sig) (methCod Sig)) methSigs)
              (DelegateReps : Fin.t DelegateIDs -> Type)
              (DelegateImpls : forall idx,
                                 ComputationalADT.pcADT (DelegateSigs idx) (DelegateReps idx))
-  : ComputationalADT.cADT (BuildADTSig consSigs methSigs) :=
+  : ComputationalADT.cADT (BuildADTSig methSigs) :=
     BuildcADT
-      (imap (Build_cConsDef (rep DelegateReps))
-            (cConstructors DelegateReps DelegateImpls))
-      (imap (Build_cMethDef (Rep:=rep DelegateReps))
+      (imap (Build_cMethDef (rep DelegateReps))
             (cMethods DelegateReps DelegateImpls)).
 
   Definition Notation_Friendly_FullySharpened_BuildMostlySharpenedcADT
              (RepT : Type)
-             {n n'}
-             {consSigs : Vector.t consSig n}
-             {methSigs : Vector.t methSig n'}
-             (consDefs : ilist consSigs)
+             {n}
+             {methSigs : Vector.t methSig n}
              (methDefs : ilist methSigs)
              (DelegateIDs : nat)
              (DelegateSigs : Fin.t DelegateIDs -> ADTSig)
              (rep : (Fin.t DelegateIDs -> Type) -> Type)
-             (cConstructors :
-                forall
-                  (DelegateReps : Fin.t DelegateIDs -> Type)
-                  (DelegateImpls : forall idx,
-                                     ComputationalADT.pcADT (DelegateSigs idx) (DelegateReps idx)),
-                  ilist
-                    (B := fun Sig : consSig =>
-                       ComputationalADT.cConstructorType
-                         (rep DelegateReps) (consDom Sig)) consSigs)
              (cMethods :
                 forall
                   (DelegateReps : Fin.t DelegateIDs -> Type)
@@ -381,7 +127,7 @@ Lemma refineADT_BuildADT_ReplaceConstructor_sigma
                   ilist
                     (B := fun Sig : methSig =>
                        ComputationalADT.cMethodType
-                         (rep DelegateReps) (methDom Sig)
+                         (methArity Sig) (rep DelegateReps) (methDom Sig)
                          (methCod Sig)) methSigs)
              (DelegateSpecs : forall idx, ADT (DelegateSigs idx))
              (cAbsR :
@@ -394,21 +140,6 @@ Lemma refineADT_BuildADT_ReplaceConstructor_sigma
                        refineADT (DelegateSpecs idx)
                                  (ComputationalADT.LiftcADT (existT _ _ (DelegateImpls idx)))),
                   RepT -> rep DelegateReps -> Prop)
-             (cConstructorsRefinesSpec : forall
-                                           (DelegateReps : Fin.t DelegateIDs -> Type)
-                                           (DelegateImpls : forall idx,
-                                                              ComputationalADT.pcADT (DelegateSigs idx) (DelegateReps idx))
-                                           (ValidImpls
-                                            : forall idx : Fin.t DelegateIDs,
-                                                refineADT (DelegateSpecs idx)
-                                                          (ComputationalADT.LiftcADT (existT _ _ (DelegateImpls idx)))),
-                 Iterate_Dep_Type_BoundedIndex
-                   (fun idx  =>
-                      @refineConstructor
-                        (RepT) (rep DelegateReps) (cAbsR _ _ ValidImpls)
-                        (consDom (Vector.nth consSigs idx))
-                        (getConsDef consDefs idx)
-                        (LiftcConstructor _ _ (ith (cConstructors DelegateReps DelegateImpls) idx))))
              (cMethodsRefinesSpec : forall
                                       (DelegateReps : Fin.t DelegateIDs -> Type)
                                       (DelegateImpls : forall idx,
@@ -422,62 +153,38 @@ Lemma refineADT_BuildADT_ReplaceConstructor_sigma
                                            @refineMethod
                                              RepT (rep DelegateReps)
                                              (cAbsR _ _ ValidImpls)
+                                             (methArity (Vector.nth methSigs idx))
                                              (methDom (Vector.nth methSigs idx))
                                              (methCod (Vector.nth methSigs idx))
                                              (getMethDef methDefs idx)
-                                             (LiftcMethod (ith (cMethods DelegateReps DelegateImpls) idx))))
-  : FullySharpenedUnderDelegates (BuildADT consDefs methDefs)
+                                             (LiftcMethod (methArity (Vector.nth methSigs idx))
+                                                          _ _ _ (ith (cMethods DelegateReps DelegateImpls) idx))))
+  : FullySharpenedUnderDelegates (BuildADT methDefs)
                                  {|
                                    Sharpened_DelegateSigs := DelegateSigs;
                                    Sharpened_Implementation := Notation_Friendly_BuildMostlySharpenedcADT
-                                                                 _ rep cConstructors cMethods;
+                                                                 _ rep cMethods;
                                    Sharpened_DelegateSpecs := DelegateSpecs |}.
   Proof.
     intros * DelegateReps DelegateImpls DelegateImplRefinesSpec.
-    eapply (@refinesADT _ (BuildADT consDefs methDefs)
+    eapply (@refinesADT _ (BuildADT methDefs)
                         (LiftcADT (existT _ (rep DelegateReps)
-                                          {| pcConstructors := _;
-                                             pcMethods := _|}))
+                                          {| pcMethods := _|}))
                         (cAbsR DelegateReps DelegateImpls DelegateImplRefinesSpec)).
-    - simpl; unfold ComputationalADT.cConstructors; simpl; intros.
-      rewrite <- ith_imap; eauto.
-      apply (Lookup_Iterate_Dep_Type
-                 _ (cConstructorsRefinesSpec DelegateReps DelegateImpls DelegateImplRefinesSpec) idx).
-        (*as [c [AbsR_c computes_c] ].
-      unfold refine; intros; inversion_by computes_to_inv; subst.
-      econstructor; eauto. *)
     - simpl; unfold ComputationalADT.cMethods; simpl; intros.
       rewrite <- ith_imap.
       apply (Lookup_Iterate_Dep_Type
                   _ (cMethodsRefinesSpec DelegateReps DelegateImpls DelegateImplRefinesSpec)).
-        (* as [r_o' [AbsR_r_o' computes_r_o'] ].
-      unfold refine; intros; inversion_by computes_to_inv; subst;
-      econstructor; eauto.
-      econstructor; eauto.
-      case_eq ((ith_Bounded methID (cMethods DelegateReps DelegateImpls) idx r_n d));
-        simpl; intros; eauto.
-      rewrite H0; eauto. *)
   Qed.
 
   Definition Notation_Friendly_SharpenFully'
              (RepT : Type)
-             {n n'}
-             (consSigs : Vector.t consSig n)
-             (methSigs : Vector.t methSig n')
-             (consDefs : ilist consSigs)
+             {n}
+             (methSigs : Vector.t methSig n)
              (methDefs : ilist methSigs)
              (DelegateIDs : nat)
              (DelegateSigs : Fin.t DelegateIDs -> ADTSig)
              (rep : (Fin.t DelegateIDs -> Type) -> Type)
-             (cConstructors :
-                forall
-                  (DelegateReps : Fin.t DelegateIDs -> Type)
-                  (DelegateImpls : forall idx,
-                                     ComputationalADT.pcADT (DelegateSigs idx) (DelegateReps idx)),
-                  ilist
-                    (B := fun Sig : consSig =>
-                       ComputationalADT.cConstructorType
-                         (rep DelegateReps) (consDom Sig)) consSigs)
              (cMethods :
                 forall
                   (DelegateReps : Fin.t DelegateIDs -> Type)
@@ -485,9 +192,10 @@ Lemma refineADT_BuildADT_ReplaceConstructor_sigma
                                      ComputationalADT.pcADT (DelegateSigs idx) (DelegateReps idx)),
                   ilist
                     (B := fun Sig : methSig =>
-                       ComputationalADT.cMethodType
-                         (rep DelegateReps) (methDom Sig)
-                         (methCod Sig)) methSigs)
+                            ComputationalADT.cMethodType
+                              (methArity Sig)
+                              (rep DelegateReps) (methDom Sig)
+                              (methCod Sig)) methSigs)
              (DelegateSpecs : forall idx, ADT (DelegateSigs idx))
              (cAbsR :
                 forall
@@ -499,21 +207,6 @@ Lemma refineADT_BuildADT_ReplaceConstructor_sigma
                        refineADT (DelegateSpecs idx)
                                  (ComputationalADT.LiftcADT (existT _ _ (DelegateImpls idx)))),
                   RepT -> rep DelegateReps -> Prop)
-             (cConstructorsRefinesSpec : forall
-                                           (DelegateReps : Fin.t DelegateIDs -> Type)
-                                           (DelegateImpls : forall idx,
-                                                              ComputationalADT.pcADT (DelegateSigs idx) (DelegateReps idx))
-                                           (ValidImpls
-                                            : forall idx : Fin.t DelegateIDs,
-                                                refineADT (DelegateSpecs idx)
-                                                          (ComputationalADT.LiftcADT (existT _ _ (DelegateImpls idx)))),
-                                           Iterate_Dep_Type_BoundedIndex
-                                             (fun idx  =>
-                                                @refineConstructor
-                                                  (RepT) (rep DelegateReps) (cAbsR _ _ ValidImpls)
-                                                  (consDom (Vector.nth consSigs idx))
-                                                  (getConsDef consDefs idx)
-                                                  (LiftcConstructor _ _ (ith (cConstructors DelegateReps DelegateImpls) idx))))
              (cMethodsRefinesSpec : forall
                                       (DelegateReps : Fin.t DelegateIDs -> Type)
                                       (DelegateImpls : forall idx,
@@ -527,20 +220,20 @@ Lemma refineADT_BuildADT_ReplaceConstructor_sigma
                                            @refineMethod
                                              RepT (rep DelegateReps)
                                              (cAbsR _ _ ValidImpls)
+                                             _
                                              (methDom (Vector.nth methSigs idx))
                                              (methCod (Vector.nth methSigs idx))
                                              (getMethDef methDefs idx)
-                                             (LiftcMethod (ith (cMethods DelegateReps DelegateImpls) idx ))))
+                                             (LiftcMethod _ _ _ _ (ith (cMethods DelegateReps DelegateImpls) idx ))))
   : FullySharpenedUnderDelegates
-      (BuildADT consDefs methDefs)
+      (BuildADT methDefs)
       {|
         Sharpened_DelegateSigs := DelegateSigs;
-        Sharpened_Implementation := Notation_Friendly_BuildMostlySharpenedcADT _ rep
-                                                                               cConstructors cMethods;
+        Sharpened_Implementation := Notation_Friendly_BuildMostlySharpenedcADT _ rep cMethods;
         Sharpened_DelegateSpecs := DelegateSpecs |} :=
-                                 (Notation_Friendly_FullySharpened_BuildMostlySharpenedcADT consDefs
-                                                                      methDefs _ rep cConstructors cMethods DelegateSpecs cAbsR
-                                                                      cConstructorsRefinesSpec cMethodsRefinesSpec).
+    (Notation_Friendly_FullySharpened_BuildMostlySharpenedcADT
+       methDefs _ rep cMethods DelegateSpecs cAbsR
+       cMethodsRefinesSpec).
 
   Record NamedDelegatee :=
     { delegateeSig : ADTSig;
@@ -568,10 +261,8 @@ Lemma refineADT_BuildADT_ReplaceConstructor_sigma
 
   Definition Notation_Friendly_SharpenFully
              (RepT : Type)
-             {m n n'}
-             (consSigs : Vector.t consSig n)
-             (methSigs : Vector.t methSig n')
-             (consDefs : ilist consSigs)
+             {m n}
+             (methSigs : Vector.t methSig n)
              (methDefs : ilist methSigs)
              (DelegateSigs' : Vector.t ADTSig m)
              (DelegateReps' : Vector.t Type m)
@@ -582,15 +273,6 @@ Lemma refineADT_BuildADT_ReplaceConstructor_sigma
              (DelegateReps := fun idx =>
                                 delegateeRep (Vector.nth Delegatees idx))
              (rep : (Fin.t DelegateIDs -> Type) -> Type)
-             (cConstructors :
-                forall
-                  (DelegateReps : Fin.t DelegateIDs -> Type)
-                  (DelegateImpls : forall idx,
-                                     ComputationalADT.pcADT (DelegateSigs idx) (DelegateReps idx)),
-                  ilist
-                    (B := fun Sig : consSig =>
-                       ComputationalADT.cConstructorType
-                         (rep DelegateReps) (consDom Sig)) consSigs)
              (cMethods :
                 forall
                   (DelegateReps : Fin.t DelegateIDs -> Type)
@@ -598,7 +280,8 @@ Lemma refineADT_BuildADT_ReplaceConstructor_sigma
                                      ComputationalADT.pcADT (DelegateSigs idx) (DelegateReps idx)),
                   ilist
                     (B := fun Sig : methSig =>
-                       ComputationalADT.cMethodType
+                            ComputationalADT.cMethodType
+                              (methArity Sig)
                          (rep DelegateReps) (methDom Sig)
                          (methCod Sig)) methSigs)
              (DelegateSpecs' : ilist (B := fun nadt => ADT (delegateeSig nadt)) Delegatees )
@@ -613,21 +296,6 @@ Lemma refineADT_BuildADT_ReplaceConstructor_sigma
                        refineADT (DelegateSpecs idx)
                                  (ComputationalADT.LiftcADT (existT _ _ (DelegateImpls idx)))),
                   RepT -> rep DelegateReps -> Prop)
-             (cConstructorsRefinesSpec : forall
-                                           (DelegateReps : Fin.t DelegateIDs -> Type)
-                                           (DelegateImpls : forall idx,
-                                                              ComputationalADT.pcADT (DelegateSigs idx) (DelegateReps idx))
-                                           (ValidImpls
-                                            : forall idx : Fin.t DelegateIDs,
-                                                refineADT (DelegateSpecs idx)
-                                                          (ComputationalADT.LiftcADT (existT _ _ (DelegateImpls idx)))),
-                                           Iterate_Dep_Type_BoundedIndex
-                                             (fun idx =>
-                                                @refineConstructor
-                                                  (RepT) (rep DelegateReps) (cAbsR _ _ ValidImpls)
-                                                  (consDom (Vector.nth consSigs idx))
-                                                  (getConsDef consDefs idx)
-                                                  (LiftcConstructor _ _ (ith (cConstructors DelegateReps DelegateImpls) idx))))
              (cMethodsRefinesSpec : forall
                                       (DelegateReps : Fin.t DelegateIDs -> Type)
                                       (DelegateImpls : forall idx,
@@ -641,25 +309,26 @@ Lemma refineADT_BuildADT_ReplaceConstructor_sigma
                                            @refineMethod
                                              RepT (rep DelegateReps)
                                              (cAbsR _ _ ValidImpls)
+                                             _
                                              (methDom (Vector.nth methSigs idx))
                                              (methCod (Vector.nth methSigs idx))
                                              (getMethDef methDefs idx)
-                                             (LiftcMethod (ith (cMethods DelegateReps DelegateImpls) idx))))
+                                             (LiftcMethod _ _ _ _ (ith (cMethods DelegateReps DelegateImpls) idx))))
   : FullySharpenedUnderDelegates
-      (BuildADT consDefs methDefs)
+      (BuildADT methDefs)
       {|
         Sharpened_DelegateSigs := DelegateSigs;
-        Sharpened_Implementation := Notation_Friendly_BuildMostlySharpenedcADT _ rep
-                                                                               cConstructors cMethods;
+        Sharpened_Implementation :=
+          Notation_Friendly_BuildMostlySharpenedcADT _ rep cMethods;
         Sharpened_DelegateSpecs := DelegateSpecs |}.
-      refine (Notation_Friendly_FullySharpened_BuildMostlySharpenedcADT consDefs
-                                                                      methDefs _ rep cConstructors cMethods DelegateSpecs cAbsR
-                                                                      cConstructorsRefinesSpec cMethodsRefinesSpec).
+    refine (Notation_Friendly_FullySharpened_BuildMostlySharpenedcADT
+              methDefs _ rep cMethods DelegateSpecs cAbsR
+              cMethodsRefinesSpec).
   Defined.
 
 End BuildADTRefinements.
 
-Arguments Notation_Friendly_BuildMostlySharpenedcADT _ _ _ _ _ _ _ _ _ _ _  / .
+Arguments Notation_Friendly_BuildMostlySharpenedcADT _ _ _ _ _ _ _ _  / .
 
 Ltac extract_delegate_free_impl :=
   cbv beta; simpl;
@@ -826,30 +495,22 @@ Ltac FullySharpenEachMethod DelegateSigs DelegateReps delegateSpecs :=
                         | Vector.t _ ?n => n
                         end in
     match goal with
-      |- FullySharpenedUnderDelegates (@BuildADT ?Rep ?n ?n' ?consSigs ?methSigs ?consDefs ?methDefs) _ =>
+      |- FullySharpenedUnderDelegates (@BuildADT ?Rep ?n ?methSigs ?methDefs) _ =>
       ilist_of_evar_dep n
-        (Fin.t NumDelegates -> Type)
-        (fun D =>
-           forall idx,
-             ComputationalADT.pcADT (delegateeSig (Vector.nth Delegatees idx)) (D idx))
-        (fun Sig => ComputationalADT.cConstructorType Rep (consDom Sig))
-        consSigs
-        ltac:(fun cCons =>
-                ilist_of_evar_dep n'
-                                  (Fin.t NumDelegates -> Type)
-                                  (fun D =>
-                                     forall idx,
-             ComputationalADT.pcADT (delegateeSig (Vector.nth Delegatees idx)) (D idx))
-        (fun Sig => ComputationalADT.cMethodType Rep (methDom Sig) (methCod Sig))
+                        (Fin.t NumDelegates -> Type)
+                        (fun D =>
+                           forall idx,
+                             ComputationalADT.pcADT (delegateeSig (Vector.nth Delegatees idx)) (D idx))
+                        (fun Sig => ComputationalADT.cMethodType Rep (methDom Sig) (methCod Sig))
         methSigs
         ltac:(fun cMeths =>
                 eapply (@Notation_Friendly_SharpenFully
-                          Rep NumDelegates n n'
-                          consSigs methSigs
-                          consDefs methDefs
+                          Rep NumDelegates n
+                          methSigs
+                          methDefs
                           DelegateSigs DelegateReps
                           (fun _ => Rep)
-                          cCons cMeths
+                          cMeths
                           delegateSpecs
                           (fun
                          (DelegateReps'' : Fin.t NumDelegates -> Type)
@@ -860,7 +521,7 @@ Ltac FullySharpenEachMethod DelegateSigs DelegateReps delegateSpecs :=
                              refineADT (DelegateSpecs idx)
                                        (ComputationalADT.LiftcADT (existT _ _ (DelegateImpls'' idx))))
                             => @eq _)
-             )))
+             ))
     end; try (simpl; repeat split; intros; subst).
 
 Ltac Implement_If_Then_Else :=
